repr/Utils.v
@@ -1,0 +1,22 @@
+From Coq Require Import Decimal String Ascii.
+Open Scope string_scope.
+
+(** [string_of_uint n] prints the uint [n] to a string in base 10. *)
+Fixpoint string_of_uint (n : uint) :=
+  match n with
+  | Nil => ""
+  | D0 n => String "0" (string_of_uint n)
+  | D1 n => String "1" (string_of_uint n)
+  | D2 n => String "2" (string_of_uint n)
+  | D3 n => String "3" (string_of_uint n)
+  | D4 n => String "4" (string_of_uint n)
+  | D5 n => String "5" (string_of_uint n)
+  | D6 n => String "6" (string_of_uint n)
+  | D7 n => String "7" (string_of_uint n)
+  | D8 n => String "8" (string_of_uint n)
+  | D9 n => String "9" (string_of_uint n)
+  end.
+
+(** [string_of_nat n] prints the natural number [n] to a string in base 10. *)
+Definition string_of_nat n : string :=
+  string_of_uint (Nat.to_uint n).
